src/Language/PlutusIR/Analysis/BoundVars/DecOpt.v
@@ -1,4 +1,5 @@
 From PlutusCert Require Import 
+  Util.In
   Util.List
   Util.DecOpt
   Language.PlutusIR
