src/Util/In.v
@@ -1,0 +1,66 @@
+From Coq Require Import
+  Strings.String
+  Lists.List.
+
+From PlutusCert Require Import 
+  Language.PlutusIR
+  Language.PlutusIR.Analysis.Equality.
+
+Import NamedTerm.
+
+
+
+(* A specialized version of In for names *)
+Inductive NameIn (x : name) : list name -> Prop :=
+  | NI_Here  : forall {xs}, NameIn x (x :: xs)
+  | NI_There : forall {x' xs}, x <> x' -> NameIn x xs -> NameIn x (x' :: xs).
+
+Lemma NameIn_In_eq : forall xs x, NameIn x xs <-> @In name x xs.
+Proof with auto using NameIn.
+  induction xs; split; intros; simpl; inversion H; subst...
+    - apply IHxs in H3...
+    - destruct (string_dec x a); subst...
+      apply NI_There... 
+      apply IHxs...
+Qed.
+
+Lemma NameIn_In_neq : forall xs x, ~ NameIn x xs <-> ~ @In name x xs.
+Proof. intros. apply not_iff_compat. apply NameIn_In_eq. Qed.
+
+
+
+(* A specialized version of In for Ty, does not require an Enum Ty instance *)
+Inductive TyIn (x : Ty) : list Ty -> Prop :=
+  | TI_Here  : forall {xs}, TyIn x (x :: xs)
+  | TI_There : forall {x' xs}, x <> x' -> TyIn x xs -> TyIn x (x' :: xs).
+
+Lemma TyIn_In_eq : forall xs x, TyIn x xs <-> @In Ty x xs.
+Proof with auto using TyIn.
+  induction xs; split; intros; simpl; inversion H; subst...
+    - apply IHxs in H3...
+    - destruct (Ty_dec x a); subst...
+      apply TI_There... 
+      apply IHxs...
+Qed.
+
+Lemma TyIn_In_neq : forall xs x, ~ TyIn x xs <-> ~ @In Ty x xs.
+Proof. intros. apply not_iff_compat. apply TyIn_In_eq. Qed.
+
+
+
+(* A specialized version of constructor for constructor *)
+Inductive ConstrIn (x : constructor) : list constructor -> Prop :=
+  | CI_Here  : forall {xs}, ConstrIn x (x :: xs)
+  | CI_There : forall {x' xs}, x <> x' -> ConstrIn x xs -> ConstrIn x (x' :: xs).
+
+Lemma ConstrIn_In_eq : forall xs x, ConstrIn x xs <-> @In constructor x xs.
+Proof with auto using ConstrIn.
+  induction xs; split; intros; simpl; inversion H; subst...
+    - apply IHxs in H3...
+    - destruct (constructor_dec x a); subst...
+      apply CI_There... 
+      apply IHxs...
+Qed.
+
+Lemma ConstrIn_In_neq : forall xs x, ~ ConstrIn x xs <-> ~ @In constructor x xs.
+Proof. intros. apply not_iff_compat. apply ConstrIn_In_eq. Qed.
